byteback-core/src/main/java/byteback/core/converter/soottoboogie/expression/Substitutor.java
@@ -9,20 +9,22 @@ import java.util.Map;
 import java.util.Optional;
 import java.util.Set;
 import soot.Local;
+import soot.Value;
+import soot.jimple.toolkits.infoflow.CachedEquivalentValue;
 
 public class Substitutor {
 
 	public final Map<Local, Expression> substitutionIndex;
 
-	public final Map<Local, Set<Local>> dependencyIndex;
+	public final Map<Value, Set<Value>> dependencyIndex;
 
-	public Substitutor(final Map<Local, Expression> substitutionIndex, final Map<Local, Set<Local>> dependencyIndex) {
+	public Substitutor(final Map<Local, Expression> substitutionIndex, final Map<Value, Set<Value>> dependencyIndex) {
 		this.substitutionIndex = substitutionIndex;
 		this.dependencyIndex = dependencyIndex;
 	}
 
-	public Substitutor(final Map<Local, Expression> substitutions) {
-		this(substitutions, new HashMap<>());
+	public Substitutor(final Map<Local, Expression> substitutionIndex) {
+		this(substitutionIndex, new HashMap<>());
 	}
 
 	public Substitutor() {
@@ -33,16 +35,25 @@ public class Substitutor {
 		return substitutionIndex;
 	}
 
-	protected void handleDependencies(final Set<Local> dependencies) {
+	protected void handleDependencies(final Set<Value> dependencies) {
 		if (dependencies.size() > 0) {
 			throw new ConversionException("Dependency found, the next substituted expressions may be invalid");
 		}
 	}
 
-	public final void put(final Local source, final Set<Local> targets, final Expression expression) {
+	public void prune(final Value dependency) {
+		final var cachedDependency = new CachedEquivalentValue(dependency);
+		if (dependencyIndex.containsKey(cachedDependency)) {
+			for (final Value source : dependencyIndex.get(cachedDependency)) {
+				substitutionIndex.remove(source);
+			}
+		}
+	}
+
+	public final void put(final Local source, final Set<Value> targets, final Expression expression) {
 		handleDependencies(dependencyIndex.getOrDefault(source, Collections.emptySet()));
 
-		for (Local target : targets) {
+		for (Value target : targets) {
 			dependencyIndex.computeIfAbsent(target, ($) -> new HashSet<>()).add(source);
 		}
 
