byteback-core/src/main/java/byteback/core/converter/soottoboogie/method/procedure/UseDefinitionCollector.java
@@ -7,18 +7,23 @@ import java.util.stream.Collectors;
 import soot.Local;
 import soot.Unit;
 import soot.toolkits.scalar.LocalDefs;
+import soot.toolkits.scalar.LocalUses;
 import soot.toolkits.scalar.SimpleLocalDefs;
+import soot.toolkits.scalar.SimpleLocalUses;
 
-public class DefinitionCollector {
+public class UseDefinitionCollector {
 
 	private Lazy<LocalDefs> definitions;
+	private Lazy<LocalUses> uses;
 
-	public DefinitionCollector() {
+	public UseDefinitionCollector() {
 		definitions = Lazy.empty();
+		uses = Lazy.empty();
 	}
 
 	public void collect(final SootBody body) {
 		definitions = Lazy.from(() -> new SimpleLocalDefs(body.getUnitGraph()));
+		uses = Lazy.from(() -> new SimpleLocalUses(body.getUnitGraph(), definitions.get()));
 	}
 
 	public boolean hasSingleDefinition(final Local local) {
@@ -31,6 +36,12 @@ public class DefinitionCollector {
 
 	public Collection<Unit> definitionsOf(final Local local) {
 		return definitions.get().getDefsOf(local).stream().collect(Collectors.toSet());
+	}
+
+	public Collection<Unit> usesOf(final Local local) {
+		return definitions.get().getDefsOf(local).stream().flatMap((unit) -> {
+			return uses.get().getUsesOf(unit).stream().map((pair) -> pair.unit).collect(Collectors.toSet()).stream();
+		}).collect(Collectors.toSet());
 	}
 
 }
