byteback-dummy/java8/src/main/java/byteback/dummy/complete/GCD.java
@@ -14,6 +14,11 @@ public class GCD {
 	}
 
 	@Condition
+	public static boolean result_decreases(int a, int b, int returns) {
+		return lte(returns, a) & lte(returns, b);
+	}
+
+	@Condition
 	public static boolean arguments_are_positive(int a, int b) {
 		return gt(a, 0) & gt(b, 0);
 	}
@@ -25,16 +30,19 @@ public class GCD {
 
 	@Condition
 	public static boolean result_divides_arguments(int a, int b, int returns) {
-		return divides(a, returns) & divides(b, returns);
+		return divides(returns, a) & divides(returns, b);
 	}
 
 	@Require("arguments_are_positive")
+	@Ensure("result_decreases")
 	@Ensure("result_is_positive")
 	@Ensure("result_divides_arguments")
 	public static int gcd(int a, int b) {
 		final int result;
 		if (a == b) {
-			return a;
+			result = a;
+			assertion(divides(result, a) & divides(result, b));
+			return result;
 		} else if (a > b) {
 			result = gcd(a - b, b);
 			return result;
