byteback-dummy/java8/src/main/java/byteback/dummy/complete/InsertionSort.java
@@ -1,0 +1,103 @@
+package byteback.dummy.complete;
+
+import static byteback.annotations.Contract.*;
+import static byteback.annotations.Operator.*;
+import static byteback.annotations.Quantifier.*;
+import static byteback.annotations.Special.*;
+
+import byteback.annotations.Binding;
+import byteback.annotations.Contract.Ensure;
+
+public class InsertionSort {
+
+	@Pure
+	public static boolean sorted(final int[] xs, int start, int end) {
+		int i = Binding.integer();
+		int j = Binding.integer();
+
+		return forall(i,
+									forall(j,
+												 implies(lte(start, i) & lt(i, j) & lt(j, end),
+																 lte(xs[i], xs[j]))));
+	}
+
+	@Pure
+	public static boolean partitioned(final int[] xs, int i, int j) {
+		int m = Binding.integer();
+		int n = Binding.integer();
+
+		return forall(m,
+									forall(n,
+												 implies(lte(0, m) & lt(m, j) & lt(j, n) & lte(n, i),
+																 lte(xs[m], xs[n]))));
+	}
+
+	@Pure
+	@Condition
+	public static boolean sorted(final int[] xs) {
+		return sorted(xs, 0, xs.length);
+	}
+
+	@Condition
+	public static boolean swapped(final int[] xs, int i, int j) {
+		return eq(xs[i], old(xs[j])) & eq(xs[j], old(xs[i]));
+	}
+
+	@Condition
+	public static boolean bounded_indexes(final int[] xs, int i, int j) {
+		return gte(i, 0) & gte(j, 0) & lt(i, xs.length) & lt(j, xs.length);
+	}
+
+	@Condition
+	public static boolean array_is_not_null(final int[] xs, int i, int j) {
+		return array_is_not_null(xs);
+	}
+
+	@Pure
+	@Condition
+	public static boolean array_is_not_null(final int[] xs) {
+		return neq(xs, null);
+	}
+
+	@Condition
+	public static boolean multi_element_array(final int[] xs) {
+		return gt(xs.length, 1);
+	}
+
+	@Require("array_is_not_null")
+	@Require("multi_element_array")
+	@Ensure("sorted")
+	public static void sort(final int[] xs) {
+		for (int i = 1; i < xs.length; ++i) {
+			invariant(lte(1, i));
+			invariant(lte(i, xs.length));
+			invariant(sorted(xs, 0, i));
+
+			for (int j = i; j > 0 && xs[j - 1] > xs[j]; --j) {
+				invariant(lte(1, i));
+				invariant(lt(i, xs.length));
+				invariant(lte(0, j));
+				invariant(lte(j, i));
+				invariant(sorted(xs, 0, j));
+				invariant(sorted(xs, j, i + 1));
+				invariant(partitioned(xs, i, j));
+
+				swap(xs, j, j - 1);
+
+				assertion(lte(xs[j], xs[i]));
+				assertion(lte(xs[j - 1], xs[j]));
+			}
+		}
+	}
+
+	@Require("array_is_not_null")
+	@Require("bounded_indexes")
+	@Ensure("swapped")
+	public static void swap(final int[] xs, int i, int j) {
+		final int y;
+		y = xs[i];
+		xs[i] = xs[j];
+		xs[j] = y;
+	}
+
+}
